thys/Monitor_Code.thy
@@ -4,8 +4,11 @@ theory Monitor_Code
   "HOL-Library.Code_Target_Nat"
   "HOL.String"
   Containers.Containers
+  SWA
 begin
 (*>*)
+
+
 
 lemma [code_unfold del, symmetric, code_post del]: "card \<equiv> Cardinality.card'" by simp
 declare [[code drop: card]] Set_Impl.card_code[code]
@@ -40,19 +43,190 @@ derive (rbt) set_impl Monitor.mregex
 derive (rbt) mapping_impl Monitor.mregex
 derive (no) cenum Monitor.mregex
 
+type_synonym 'a msaux = "nat \<times> \<I> \<times> (ts \<times> 'a table) list"
+
+global_interpretation default: msaux
+  "\<lambda>w (nt, I, xs) ys. I = ivl w \<and> current w = nt \<and> xs = ys"
+  "\<lambda>I. (0, I, [] :: (ts \<times> 'a table) list)"
+  "\<lambda>nt (t, I, xs). (t, I, filter (\<lambda>(t, X). enat (nt - t) \<le> right I) xs)"
+  "\<lambda>pos rel1 (t, I, xs). (t, I, map (\<lambda>(t, X). (t, join X pos rel1)) xs)"
+  "\<lambda>(nt, X) (t, I, xs). (nt, I, case xs of [] \<Rightarrow> [(nt, X)]
+    | (t, Y) # ts \<Rightarrow> if t = nt then (nt, Y \<union> X) # ts else (nt, X) # xs)"
+  "\<lambda>(nt, I, xs). foldr (\<union>) [rel. (t, rel) \<leftarrow> xs, nt - t \<ge> left I] {}"
+  defines minit0 = "msaux.minit0 (\<lambda>I. (0, I, [] :: (ts \<times> 'a table) list)) :: nat \<Rightarrow> 'a Formula.formula \<Rightarrow> ( 'a msaux, 'a) mformula"
+  and minit = "msaux.minit (\<lambda>I. (0, I, [] :: (ts \<times> 'a table) list)):: 'a Formula.formula \<Rightarrow> ( 'a msaux, 'a) mstate"
+  and minit_safe = "msaux.minit_safe (\<lambda>I. (0, I, [] :: (ts \<times> 'a table) list)) :: 'a Formula.formula \<Rightarrow> ( 'a msaux, 'a) mstate"
+  and update_since = "msaux.update_since
+    (\<lambda>nt (t, I, xs). (t, I, filter (\<lambda>(t, X). enat (nt - t) \<le> right I) xs))
+    (\<lambda>pos rel1 (t, I, xs). (t, I, map (\<lambda>(t, X). (t, join X pos rel1)) xs))
+    (\<lambda>(nt, X) (t, I, xs). (nt, I, case xs of [] \<Rightarrow> [(nt, X)]
+    | (t, Y) # ts \<Rightarrow> if t = nt then (nt, Y \<union> X) # ts else (nt, X) # xs))
+    (\<lambda>(nt, I, xs). foldr (\<union>) [rel. (t, rel) \<leftarrow> xs, nt - t \<ge> left I] {})"
+  and meval = "msaux.meval
+    (\<lambda>nt (t, I, xs). (t, I, filter (\<lambda>(t, X). enat (nt - t) \<le> right I) xs))
+    (\<lambda>pos rel1 (t, I, xs). (t, I, map (\<lambda>(t, X). (t, join X pos rel1)) xs))
+    (\<lambda>(nt, X) (t, I, xs). (nt, I, case xs of [] \<Rightarrow> [(nt, X)]
+    | (t, Y) # ts \<Rightarrow> if t = nt then (nt, Y \<union> X) # ts else (nt, X) # xs))
+    (\<lambda>(nt, I, xs). foldr (\<union>) [rel. (t, rel) \<leftarrow> xs, nt - t \<ge> left I] {})"
+  and mstep = "msaux.mstep
+    (\<lambda>nt (t, I, xs). (t, I, filter (\<lambda>(t, X). enat (nt - t) \<le> right I) xs))
+    (\<lambda>pos rel1 (t, I, xs). (t, I, map (\<lambda>(t, X). (t, join X pos rel1)) xs))
+    (\<lambda>(nt, X) (t, I, xs). (nt, I, case xs of [] \<Rightarrow> [(nt, X)]
+    | (t, Y) # ts \<Rightarrow> if t = nt then (nt, Y \<union> X) # ts else (nt, X) # xs))
+    (\<lambda>(nt, I, xs). foldr (\<union>) [rel. (t, rel) \<leftarrow> xs, nt - t \<ge> left I] {})"
+  and msteps0_stateless = "msaux.msteps0_stateless
+    (\<lambda>nt (t, I, xs). (t, I, filter (\<lambda>(t, X). enat (nt - t) \<le> right I) xs))
+    (\<lambda>pos rel1 (t, I, xs). (t, I, map (\<lambda>(t, X). (t, join X pos rel1)) xs))
+    (\<lambda>(nt, X) (t, I, xs). (nt, I, case xs of [] \<Rightarrow> [(nt, X)]
+    | (t, Y) # ts \<Rightarrow> if t = nt then (nt, Y \<union> X) # ts else (nt, X) # xs))
+    (\<lambda>(nt, I, xs). foldr (\<union>) [rel. (t, rel) \<leftarrow> xs, nt - t \<ge> left I] {})"
+  and msteps_stateless = "msaux.msteps_stateless
+    (\<lambda>nt (t, I, xs). (t, I, filter (\<lambda>(t, X). enat (nt - t) \<le> right I) xs))
+    (\<lambda>pos rel1 (t, I, xs). (t, I, map (\<lambda>(t, X). (t, join X pos rel1)) xs))
+    (\<lambda>(nt, X) (t, I, xs). (nt, I, case xs of [] \<Rightarrow> [(nt, X)]
+    | (t, Y) # ts \<Rightarrow> if t = nt then (nt, Y \<union> X) # ts else (nt, X) # xs))
+    (\<lambda>(nt, I, xs). foldr (\<union>) [rel. (t, rel) \<leftarrow> xs, nt - t \<ge> left I] {})"
+  and monitor = "msaux.monitor (\<lambda>I. (0, I, []))
+    (\<lambda>nt (t, I, xs). (t, I, filter (\<lambda>(t, X). enat (nt - t) \<le> right I) xs))
+    (\<lambda>pos rel1 (t, I, xs). (t, I, map (\<lambda>(t, X). (t, join X pos rel1)) xs))
+    (\<lambda>(nt, X) (t, I, xs). (nt, I, case xs of [] \<Rightarrow> [(nt, X)]
+    | (t, Y) # ts \<Rightarrow> if t = nt then (nt, Y \<union> X) # ts else (nt, X) # xs))
+    (\<lambda>(nt, I, xs). foldr (\<union>) [rel. (t, rel) \<leftarrow> xs, nt - t \<ge> left I] {})"
+  by unfold_locales (auto simp: init_window_def split: list.splits)
+(*
+(*
+definition update_since :: "\<I> \<Rightarrow> bool \<Rightarrow> 'a table \<Rightarrow> 'a table \<Rightarrow> ts \<Rightarrow>
+  'a msaux \<Rightarrow> 'a table \<times> 'a msaux" where
+  "update_since I pos rel1 rel2 nt aux =
+    (let auxrest0 = [(t, join rel pos rel1). (t, rel) \<leftarrow> snd aux];
+         auxrest0' = (case auxrest0 of
+             [] \<Rightarrow> (nt, rel2) # map (\<lambda>i. (i, empty_table)) (rev [r (fst aux) ..< nt])
+           | x # aux' \<Rightarrow> (if fst x = nt then (fst x, snd x \<union> rel2) # aux'
+              else (nt, rel2) # map (\<lambda>i. (i, empty_table)) (rev [Suc (fst x) ..< nt]) @ (x # aux')));
+         auxtree0 = map_tree (\<lambda>rel. join rel pos rel1) (fst aux);
+         auxtree' =
+           (if r auxtree0 = Suc nt then
+              update_rightmost (\<lambda>rel. rel + rel2) auxtree0
+            else if Suc nt - left I > 0 then
+              (let window = (max 1 (the_enat (enat (Suc nt) - right I)), Suc nt - left I);
+                   new_atoms = drop (left I) auxrest0'
+               in slide' (rev (map snd new_atoms)) auxtree0 window)
+            else auxtree0)
+     in (if Suc nt - left I > 0 then the (val auxtree') else empty_table, (auxtree', take (left I) auxrest0')))"
+*)
+
+(*
+  "wf_since_aux \<sigma> n R pos \<phi> I \<psi> aux ne \<longleftrightarrow>
+    (\<exists>auxlist.
+      l (fst aux) = (if ne = 0 then 0 else if Suc (\<tau> \<sigma> (ne-1)) - left I > 0 then max 1 (the_enat (enat (Suc (\<tau> \<sigma> (ne-1))) - right I)) else 0) \<and>
+      r (fst aux) = (if ne = 0 then 0 else Suc (\<tau> \<sigma> (ne-1)) - left I) \<and>
+      take (left I) auxlist = snd aux \<and>
+      valid (replicate (l (fst aux) - 1) empty_table @ rev (map snd (drop (left I) auxlist))) (fst aux) \<and>
+      sorted_wrt (\<lambda>x y. fst x > fst y) auxlist \<and>
+      (\<forall>t X. (t, X) \<in> set auxlist \<longrightarrow> ne \<noteq> 0 \<and> t \<le> \<tau> \<sigma> (ne-1) \<and> \<tau> \<sigma> (ne-1) - t \<le> right I \<and>
+        (if (\<exists>i. \<tau> \<sigma> i = t) then qtable n (MFOTL.fv \<psi>) (mem_restr R) (\<lambda>v. MFOTL.sat \<sigma> (map the v) (ne-1) (Sincep pos \<phi> (point (\<tau> \<sigma> (ne-1) - t)) \<psi>)) X else X = empty_table)) \<and>
+      (\<forall>t. ne \<noteq> 0 \<and> t \<le> \<tau> \<sigma> (ne-1) \<and> \<tau> \<sigma> (ne-1) - t \<le> right I \<longrightarrow>
+        (\<exists>X. (t, X) \<in> set auxlist)))"
+*)
+fun fill where
+  "fill ((t, X) # (u, Y) # xs) = (t, X) # map (\<lambda>t. (t, empty_table)) [t + 1 ..< u] @ fill ((u, Y) # xs)"
+| "fill xs = xs"
+
+lemma join_empty_table[simp]: "join empty_table pos rel = empty_table"
+  by (auto simp: Table.join_def empty_table_def)
+
+lemma map_join_fill:
+  "map (\<lambda>(t, X). (t, join X pos rel)) (fill xs) = fill (map (\<lambda>(t, X). (t, join X pos rel)) xs)"
+  by (induct xs rule: fill.induct) (auto simp: drop_Cons' gr0_conv_Suc drop_map)
+
+lemma map_join_take_fill:
+  "map (\<lambda>(t, X). (t, join X pos rel)) (take n (fill xs)) = take n (fill (map (\<lambda>(t, X). (t, join X pos rel)) xs))"
+  by (auto simp: take_map[symmetric] map_join_fill)
+
+lemma map_join_drop_fill:
+  "map (\<lambda>(t, X). (t, join X pos rel)) (drop n (fill xs)) = drop n (fill (map (\<lambda>(t, X). (t, join X pos rel)) xs))"
+  by (auto simp: drop_map[symmetric] map_join_fill)
+
+lemma join_distr: "join (A \<union> B) pos C = join A pos C \<union> join B pos C"
+  by (cases pos) (auto simp: join_False_code join_True_code)
+
+lemma map_snd_flip: "map f (map snd xs) = map snd (map (\<lambda>(a, b). (a, f b)) xs)"
+  by (auto simp: list.map_comp fun_eq_iff)
+
+global_interpretation swa: msaux
+  "\<lambda>w (I, t, xs) ys.
+     let auxlist = fill ys in
+     ivl w = I \<and>
+     current w = r t + length xs - Suc 0 \<and>
+     take (left (ivl w)) auxlist = xs \<and>
+     valid (replicate (l t - 1) empty_table @ rev (map snd (drop (left (ivl w)) auxlist))) t \<and>
+     l t = (if t = Leaf then 0 else earliest w + Suc 0) \<and>
+     r t = (if t = Leaf then 0 else latest w + Suc 0)"
+  "\<lambda>I. (I, Leaf, [])"
+  "undefined"
+  "\<lambda>pos rel (I, t, xs). (I, map_tree (\<lambda>X. join X pos rel) t, map (\<lambda>(t, X). (t, join X pos rel)) xs)"
+  "\<lambda>(nt, X) (I, t, xs).
+    let xs' =
+      (case xs of [] \<Rightarrow> (nt, X) # map (\<lambda>i. (i, empty_table)) (rev [r t ..< nt])
+           | x # aux' \<Rightarrow> (if fst x = nt then (fst x, snd x \<union> X) # aux'
+              else (nt, X) # map (\<lambda>i. (i, empty_table)) (rev [Suc (fst x) ..< nt])));
+      t' = (if r t = Suc nt then
+              update_rightmost (\<lambda>rel. rel + X) t
+            else if Suc nt - left I > 0 then
+              (let window = (max 1 (the_enat (enat (Suc nt) - right I)), Suc nt - left I);
+                   new_atoms = drop (left I) xs'
+               in slide' (rev (map snd new_atoms)) t window)
+            else t)
+    in (I, t', xs')"
+  "\<lambda>(I, t, xs). case val t of None \<Rightarrow> empty_table | Some X \<Rightarrow> X"
+  apply unfold_locales
+  subgoal by (auto simp: valid_Leaf init_window_def)
+  subgoal sorry
+  subgoal for w msaux auxlist pos rel
+    by (auto simp: valid_Leaf Let_def map_join_take_fill map_join_drop_fill map_join_fill[symmetric]
+      join_distr plus_set_def rev_map[symmetric] map_snd_flip simp del: map_map
+      dest!: valid_map_map_tree[where f="\<lambda>X. join X pos rel" and as = "replicate (earliest w) empty_table @ rev (map snd (drop (left (ivl w)) (fill auxlist)))", rotated])
+  subgoal sorry
+  subgoal for w msaux auxlist
+    apply (auto split: option.splits if_splits simp: Let_def)
+       apply (frule val_eq_Some_sum_if_valid_neq_Leaf)
+        apply auto []
+       apply (subst (asm) sum_alt)
+         apply simp
+        apply (unfold valid_def)
+        apply (case_tac a)
+         apply auto [2]
+         apply (auto simp: rev_filter[symmetric] filter_map o_def nth_append empty_table_def plus_set_def zero_set_def split: if_split) []
+       apply (simp add: foldr_conv_fold plus_set_def zero_set_def del: fold_simps)
+       apply (erule arg_cong[where f="\<lambda>x. _ \<in> x", THEN iffD1, rotated])
+       apply (rule arg_cong[where f="\<lambda>xs. fold (\<union>) (rev xs) {}"])
+    apply (rule nth_equalityI)
+        apply auto []
+    find_theorems "concat (map _ _)"
+    thm fold_plus_sum_list_rev
+(*
+    apply simp
+      apply (auto dest!: val_eq_Some_sum_if_valid_neq_Leaf simp: nth_append
+        rev_map[symmetric] foldr_conv_fold fold_plus_sum_list_rev split: if_splits)
+*)
+    find_theorems "fold (+)"
+    sorry
+  done
+*)
+
 lemma image_these: "f ` Option.these X = Option.these (map_option f ` X)"
   by (force simp: in_these_eq Bex_def image_iff map_option_case split: option.splits)
 
 lemma meval_MPred: "meval n t db (MPred e ts) = ([Option.these
   ((map_option (\<lambda>f. Table.tabulate f 0 n) o match ts) ` (\<Union>(e', x)\<in>db. if e = e' then {x} else {}))], MPred e ts)"
-  unfolding meval.simps image_these image_image o_def ..
+  unfolding default.meval.simps image_these image_image o_def ..
 
 lemma meval_MPred': "meval n t db (MPred e ts) = ([Option.these
   (\<Union>(e', x)\<in>db. if e = e' then {map_option (\<lambda>f. Table.tabulate f 0 n) (match ts x)} else {})], MPred e ts)"
   unfolding meval_MPred image_UN split_beta if_distrib[of "image _"] image_insert image_empty o_apply
   ..
 
-lemma these_UNION: "Option.these (UNION A B) = UNION A (Option.these o B)"
+lemma these_UNION: "Option.these (\<Union>x \<in> A. B x) = (\<Union>x \<in> A. (Option.these o B) x)"
   by (auto simp: Option.these_def)
 
 lemma meval_MPred'': "meval n t db (MPred e ts) = ([
@@ -60,7 +234,7 @@ lemma meval_MPred'': "meval n t db (MPred e ts) = ([
   unfolding meval_MPred' these_UNION o_def prod.case_distrib[of Option.these]
   by (auto simp: Option.these_def map_option_case image_iff split: if_splits option.splits)
 
-lemmas meval_code[code] = meval.simps(1) meval_MPred'' meval.simps(3-13)
+lemmas meval_code[code] = default.meval.simps(1) meval_MPred'' default.meval.simps(3-13)
 
 definition mk_db :: "(char list \<times> 'a list) list \<Rightarrow> (char list \<times> 'a list) set" where
   "mk_db = set"
@@ -100,7 +274,7 @@ declare RPDs_code[code del]
 lemma RPDs_code[code]: "RPDs r = RPDs_aux {r}"
   unfolding RPDs_aux_def RPDs_code
   by (rule saturate_commute[where C="RPDs r"])
-     (auto simp: mono_def subset_singleton_iff RPDs_refl RPDs_trans finite_RPDs)
+     (auto 0 3 simp: mono_def subset_singleton_iff RPDs_refl RPDs_trans finite_RPDs)
 
 definition "LPDs_aux = saturate (\<lambda>S. S \<union> \<Union> (LPD ` S))"
 
@@ -113,7 +287,7 @@ declare LPDs_code[code del]
 lemma LPDs_code[code]: "LPDs r = LPDs_aux {r}"
   unfolding LPDs_aux_def LPDs_code
   by (rule saturate_commute[where C="LPDs r"])
-     (auto simp: mono_def subset_singleton_iff LPDs_refl LPDs_trans finite_LPDs)
+     (auto 0 3 simp: mono_def subset_singleton_iff LPDs_refl LPDs_trans finite_LPDs)
 
 lemma is_empty_table_unfold [code_unfold]:
   "X = empty_table \<longleftrightarrow> Set.is_empty X"
@@ -124,10 +298,10 @@ lemma is_empty_table_unfold [code_unfold]:
   "set_eq empty_table X \<longleftrightarrow> Set.is_empty X"
   unfolding set_eq_def empty_table_def Set.is_empty_def Cardinality.eq_set_def by auto
 
-lemma tabulate_rbt_code[code]: "Monitor.tabulate (xs :: 'a :: ccompare list) f =
-  (case ID CCOMPARE('a) of None \<Rightarrow> Code.abort (STR ''tabulate RBT_Mapping: ccompare = None'') (\<lambda>_. Monitor.tabulate (xs :: 'a :: ccompare list) f)
+lemma tabulate_rbt_code[code]: "Monitor.mrtabulate (xs :: mregex list) f =
+  (case ID CCOMPARE(mregex) of None \<Rightarrow> Code.abort (STR ''tabulate RBT_Mapping: ccompare = None'') (\<lambda>_. Monitor.mrtabulate (xs :: mregex list) f)
   | _ \<Rightarrow> RBT_Mapping (RBT_Mapping2.bulkload (List.map_filter (\<lambda>k. let fk = f k in if fk = empty_table then None else Some (k, fk)) xs)))"
-  unfolding tabulate.abs_eq RBT_Mapping_def
+  unfolding mrtabulate.abs_eq RBT_Mapping_def
   by (auto split: option.splits)
 
 export_code convert_multiway minit_safe mstep
